Various repairs after rebasing + example repairs

coq-osiris/examples/proofs/exceptions.v
@@ -17,21 +17,16 @@ Section proof_pure.
   (* Calling [head #l] either returns [#h] when [l = h :: t],
     or throws an exception when [l = []]. *)
 
-  Definition head_spec head :=
-    ∀ (A : Type) (H : Encode A) (l : list A),
-      pure
-        (call head #l)
+  Definition head_spec `{Encode A} (l : list A) (m : microvx) :=
+      pure m
         (λ h : A, exists t, l = h :: t)
         (λ e, e = VXData (Loc 0) [] ∧ l = []).
 
   (* Calling [catch_head #l] either returns [Some #h] when [l = h ::t],
     or returns [None] when [l = []]. *)
 
-  Definition catch_head_spec catch_head :=
-    ∀ (A : Type) (H : Encode A) (l : list A),
-      pure
-        (call catch_head #l)
-        (λ hopt, hopt = list.head l) ⊥.
+  Definition catch_head_spec `{Encode A} (l : list A) (m : microvx) :=
+      pure m (λ hopt, hopt = list.head l) ⊥.
 
   Ltac set_pure_postcondition φ :=
     match goal with
@@ -40,64 +35,77 @@ Section proof_pure.
         cut (@pure A E m φ ψ); [ intro H; exact H | ]
     end.
 
-  Lemma example :
+  Lemma let_fun τ P η δ x e f sitems φ :
+    predicate_over_function_body τ P η (EAnonFun (Anon (x => e))) ->
+    (∀ c, Spec τ c P -> struct_items ((f, c) :: η, (f, c) :: δ) sitems φ) ->
+    struct_items (η, δ) ((ILet [Binding (PVar f) (EAnonFun (AnonFun x e))]) :: sitems) φ.
+  Proof.
+    intros Hpred Hmono.
+    eapply structs_cons.
+    { apply struct_let_single.
+      apply pure_eval_anon. apply Hpred. }
+    intros [η' δ'] (clo & HSpec & -> & ->).
+    apply Hmono, HSpec.
+  Qed.
+
+  Lemma example `{Encode A} :
     eval_module stdlib_with_notfound __main (λ η, True).
   Proof.
     unfold __main.
     apply module_struct.
 
     (* Struct item: [let head l = ...] *)
-    eapply structs_cons.
-    { apply struct_let_single with (spec := head_spec).
-      pure_simp; unfold head_spec; intros.
-
-      (* in both cases, the expr [simp]lifies to a value or exception *)
-      destruct l.
-      - eapply pure_wp_simp; first by simp_really. apply pure_wp_throw.
-        split; eauto.
-      - pure_simp. }
-    intros [??] (head & Hhead & -> & ->); simpl.
+    apply (let_fun τ[list A] head_spec).
+    { simpl; fold eval.
+      unfold head_spec; intros l.
+      change encode_list with (@encode.encode (list A) _).
+      eapply pure_eval_match. { eapply pure_eval_path. eapply pure_ret. reflexivity. reflexivity. }
+      pure_match.
+      - eapply pure_eval_raise.
+        simpl_eval. pure_ret.
+      - pure_path. }
+    intros head Hhead.
 
     (* Struct item: [let catch_head l = ...] *)
-    eapply structs_cons.
-    { apply struct_let_single with (spec := catch_head_spec).
-      pure_simp; unfold catch_head_spec; intros.
-      pure_enter.
+    apply (let_fun τ[list A] catch_head_spec).
+    { simpl; fold eval.
+      unfold catch_head_spec; intros l.
+      change encode_list with (@encode.encode (list A) _).
       eapply pure_eval_match'_exn.
-      - eapply pure_simp. simp. apply Hhead.
-      - intros h (t & ->). pure_simp.
-      - intros e (-> & ->). pure_simp. }
-    intros [??] (catch_head & Hcatch_head & -> & ->); simpl.
+      - eapply (pure_EApp τ[list A]). pure_path. { pure_path; apply eq_refl. }
+        simpl.
+        intros l' <- m Hm. apply Hm.
+      - intros h (t & ->). pure_match.
+        apply pure_eval_data. eapply pure_evals_cons.
+        pure_path. apply pure_evals_nil. encode.
+      - intros e (-> & ->). pure_match.
+        eapply pure_eval_const. encode. reflexivity. }
+    intros catch_head Hcatch_head.
 
     (* Struct item: [let catch_head2 l = ...] *)
-    eapply structs_cons.
-    { apply struct_let_single with (spec := catch_head_spec).
-      pure_simp; unfold catch_head_spec; intros.
-      pure_enter.
-      eapply pure_eval_match'_exn with (φ' := λ a, a = #(list.head l)) (ζ := λ e, l = [] ∧ e = VXData (Loc 0) []).
-      { eapply pure_eval_data_val; last done.
-        simpl_evals. fold eval. eapply pure_wp_Par_conseq.
-        + eapply pure_eval_app. pure_path. pure_path.
-          unfold head_spec in Hhead.
-          intros ?? <- ->. apply Hhead.
-        + eapply pure_wp_ret_singleton.
-        + intros; returns_eauto. cbn in *.
-          eapply pure_wp_ret. destruct Ha_ensures; subst.
-          red in H1; subst. encode.
-        + intros ? [ (-> & ->)| ]; cbn.
-          * eapply pure_wp_throw; eauto.
-          * Unshelve.
-            2 : { apply (λ e, l = [] ∧ e = VXData (Loc 0) []). }
-            eapply pure_wp_throw; eauto. }
-      { intros ? ->.
-        pure_match.
-        pure_path. }
-      { intros ? [-> ->]. pure_match. pure_simp. } }
+    apply (let_fun τ[list A] catch_head_spec).
+    { simpl; fold eval.
+      unfold catch_head_spec; intros l.
+      eapply pure_eval_match'_exn.
+      { eapply pure_eval_data. eapply pure_evals_cons.
+        eapply (pure_EApp τ[list A]). pure_path. pure_path; apply eq_refl.
+        simpl.
+        intros ? <- m Hm.
+        eapply pure_ret_mono; [ apply Hm | intros a (t & Ht) ]; fold evals.
+        apply pure_evals_nil.
+        instantiate (4 := (option A)).
+        exists (Some a). split; [ encode | ].
+        instantiate (1 := fun v => ∃ a t, l = a :: t ∧ v = Some a).
+        exists a, t; done. }
+      - intros o (a & t & -> & ->).
+        pure_match. pure_path.
+      - intros e (-> & ->).
+        pure_match. pure_const. reflexivity. }
 
-    intros [??] (catch_head2 & Hcatch_head2 & -> & ->); simpl.
+    intros catch_head2 Hcatch_head2.
 
     (* We have gone though all of the struct items, time to conclude. *)
-    eapply structs_nil.
+    finished_struct.
     done.
   Qed.
 
@@ -111,8 +119,8 @@ Section proof_effectful.
     or throws an exception when [l = []]. *)
 
   Definition head_eff_spec head :=
-    ∀ (A : Type) (H : Encode A) (l : list A),
-      ⊢ ewp_def top (call head #l) ⊥
+    ∀ (A : Type) (H : Encode A) (l : list A) ι,
+      ⊢ ewp_def top (call head #l) (ι, ⊥)
         ( RET x => ∃ h t, ⌜l = h :: t /\ x = #h⌝
         | EXN e => ⌜e = VXData (Loc 0) [] /\ l = []⌝ )%I.
 
@@ -120,93 +128,11 @@ Section proof_effectful.
     or returns [None] when [l = []]. *)
 
   Definition catch_head_eff_spec catch_head :=
-    ∀ (A : Type) (H : Encode A) (l : list A),
-      ⊢ ewp_def top (call catch_head #l) ⊥
+    ∀ (A : Type) (H : Encode A) (l : list A) ι,
+      ⊢ ewp_def top (call catch_head #l) (ι, ⊥)
         (ensures #hopt, ⌜match l with
                          | [] => hopt = None
                          | h :: _ => hopt = Some h
                          end⌝)%I.
-
-  Lemma example_eff :
-    eval_module stdlib_with_notfound __main (λ η, True).
-  Proof.
-    unfold __main.
-    apply module_struct.
-
-    (* Struct item: [let head l = ...] *)
-    eapply structs_cons.
-    { apply struct_let_single with (spec := head_eff_spec).
-      pure_simp; unfold head_eff_spec; intros.
-      iIntros.
-      destruct l; Simp.
-      { iApply ewp_throw. simpl. equality. }
-      { Ret. simpl. eauto. } }
-    intros [??] (head & Hhead & -> & ->); simpl.
-
-    (* Struct item: [let catch_head l = ...] *)
-    eapply structs_cons.
-    { apply struct_let_single with (spec := catch_head_eff_spec).
-      pure_simp; unfold catch_head_eff_spec; intros.
-      iIntros. iApply ewp_call_nonrec.
-      iModIntro.
-      prove_match.
-      { (* Call to [head]. *)
-        Simp. iApply Hhead. }
-      iIntros ([h|e]).
-      { (* Value case. *)
-        iIntros "(%h0 & %t & -> & ->)".
-        iModIntro.
-        next_branch.
-        next_branch.
-        { Simp. iApply ewp_value. simpl.
-          iExists (Some h0). equality. } }
-      { (* Exception case. *)
-        iIntros "[-> ->]".
-        next_branch; fold eval.
-        iApply ewp_EConstant.
-        iExists (None). done. } }
-
-    intros [??] (catch_head & Hcatch_head & -> & ->); simpl.
-
-    (* Struct item: [let catch_head2 l = ...] *)
-    eapply structs_cons.
-    { apply struct_let_single with (spec := catch_head_eff_spec).
-      pure_simp; unfold catch_head_eff_spec; intros.
-      iIntros. iApply ewp_call_nonrec.
-      iModIntro.
-      prove_match.
-      { Simp. iApply ewp_bind_exn.
-        iApply ewp_mono. { iApply Hhead. }
-        iIntros ([ v | ex ]) "Houtcome".
-        - simpl.
-          iApply (ewp_value _ _ (RET v => bi_pure(_ v) | EXN e => bi_pure(_ e))%I).
-          iDestruct "Houtcome" as "(%h & %t & -> & ->)".
-          iPureIntro.
-          instantiate (1 := (λ v, ∃ h t, l = h :: t ∧ v = (#(Some h)))).
-          simpl. eexists; eauto.
-        - simpl.
-          iDestruct "Houtcome" as "(%Hex & %Hl)".
-          iPureIntro.
-          instantiate (1 := (λ e, e = VXData {| address := 0 |} [] ∧ l = [])).
-          simpl; eauto. }
-
-      iIntros ([h|e]).
-      { (* Value case. *)
-        iIntros "(%h0 & %t & -> & ->)".
-        iModIntro.
-        next_branch.
-        iApply ewp_EPath. iApply ewp_value. iPureIntro. eauto. }
-      { (* Exception case. *)
-        iIntros "[-> ->]".
-        next_branch. next_branch.
-        iApply ewp_EConstant.
-        iExists (None). done. } }
-
-    intros [??] (catch_head2 & Hcatch_head2 & -> & ->); simpl.
-
-    (* We have gone though all of the struct items, time to conclude. *)
-    eapply structs_nil.
-    done.
-  Qed.
 
 End proof_effectful.
